proofs/fstar/extraction/Bertie.Tls13formats.fsti
@@ -858,6 +858,7 @@ val parse_server_hello
 
 val check_extensions_slice (algs: Bertie.Tls13crypto.t_Algorithms) (b: t_Slice u8)
     : Prims.Pure (Core.Result.t_Result t_Extensions u8) Prims.l_True (fun _ -> Prims.l_True)
+     (decreases Seq.length b)
 
 val check_extensions (algs: Bertie.Tls13crypto.t_Algorithms) (b: Bertie.Tls13utils.t_Bytes)
     : Prims.Pure (Core.Result.t_Result t_Extensions u8) Prims.l_True (fun _ -> Prims.l_True)
